theories/Numbers/HexadecimalQ.v
@@ -19,53 +19,86 @@ Require Import Hexadecimal HexadecimalFacts HexadecimalPos HexadecimalN Hexadeci
 Lemma of_to (q:IQ) : forall d, to_hexadecimal q = Some d -> of_hexadecimal d = q.
 Admitted.
 
-(* normalize without fractional part, for instance norme 0x1.2p-1 is 0x12e-5 *)
-Definition hnorme (d:hexadecimal) : hexadecimal :=
-  let '(i, f, e) :=
-    match d with
-    | Hexadecimal i f => (i, f, Decimal.Pos Decimal.Nil)
-    | HexadecimalExp i f e => (i, f, e)
+Definition dnorm (d:hexadecimal) : hexadecimal :=
+  let norm_i i f :=
+    match i with
+    | Pos i => Pos (unorm i)
+    | Neg i => match nzhead (app i f) with Nil => Pos zero | _ => Neg (unorm i) end
     end in
-  let i := norm (app_int i f) in
-  let e := (Z.of_int e - 4 * Z.of_nat (nb_digits f))%Z in
-  match e with
-  | Z0 => Hexadecimal i Nil
-  | Zpos e => Hexadecimal (Pos.iter double i e) Nil
-  | Zneg _ => HexadecimalExp i Nil (Decimal.norm (Z.to_int e))
+  match d with
+  | Hexadecimal i f => Hexadecimal (norm_i i f) f
+  | HexadecimalExp i f e =>
+    match Decimal.norm e with
+    | Decimal.Pos Decimal.zero => Hexadecimal (norm_i i f) f
+    | e => HexadecimalExp (norm_i i f) f e
+    end
   end.
 
-Lemma hnorme_spec d :
-  match hnorme d with
-  | Hexadecimal i Nil => i = norm i
-  | HexadecimalExp i Nil e =>
-    i = norm i /\ e = Decimal.norm e /\ e <> Decimal.Pos Decimal.zero
-  | _ => False
+Lemma dnorm_spec_i d :
+  let (i, f) :=
+    match d with Hexadecimal i f => (i, f) | HexadecimalExp i f _ => (i, f) end in
+  let i' := match dnorm d with Hexadecimal i _ => i | HexadecimalExp i _ _ => i end in
+  match i with
+  | Pos i => i' = Pos (unorm i)
+  | Neg i =>
+    (i' = Neg (unorm i) /\ (nzhead i <> Nil \/ nzhead f <> Nil))
+    \/ (i' = Pos zero /\ (nzhead i = Nil /\ nzhead f = Nil))
   end.
 Admitted.
 
-Lemma hnorme_invol d : hnorme (hnorme d) = hnorme d.
+Lemma dnorm_spec_f d :
+  let f := match d with Hexadecimal _ f => f | HexadecimalExp _ f _ => f end in
+  let f' := match dnorm d with Hexadecimal _ f => f | HexadecimalExp _ f _ => f end in
+  f' = f.
 Admitted.
 
-Lemma to_of (d:hexadecimal) :
-  to_hexadecimal (of_hexadecimal d) = Some (hnorme d).
+Lemma dnorm_spec_e d :
+  match d, dnorm d with
+    | Hexadecimal _ _, Hexadecimal _ _ => True
+    | HexadecimalExp _ _ e, Hexadecimal _ _ =>
+      Decimal.norm e = Decimal.Pos Decimal.zero
+    | HexadecimalExp _ _ e, HexadecimalExp _ _ e' =>
+      e' = Decimal.norm e /\ e' <> Decimal.Pos Decimal.zero
+    | Hexadecimal _ _, HexadecimalExp _ _ _ => False
+  end.
+Admitted.
+
+Lemma dnorm_invol d : dnorm (dnorm d) = dnorm d.
+Admitted.
+
+Lemma to_of (d:hexadecimal) : to_hexadecimal (of_hexadecimal d) = Some (dnorm d).
 Admitted.
 
 (** Some consequences *)
 
 Lemma to_hexadecimal_inj q q' :
   to_hexadecimal q <> None -> to_hexadecimal q = to_hexadecimal q' -> q = q'.
-Admitted.
+Proof.
+intros Hnone EQ.
+generalize (of_to q) (of_to q').
+rewrite <-EQ.
+revert Hnone; case to_hexadecimal; [|now simpl].
+now intros d _ H1 H2; rewrite <-(H1 d eq_refl), <-(H2 d eq_refl).
+Qed.
 
-Lemma to_hexadecimal_surj d : exists q, to_hexadecimal q = Some (hnorme d).
-Admitted.
+Lemma to_hexadecimal_surj d : exists q, to_hexadecimal q = Some (dnorm d).
+Proof.
+  exists (of_hexadecimal d). apply to_of.
+Qed.
 
-Lemma of_hexadecimal_hnorme d : of_hexadecimal (hnorme d) = of_hexadecimal d.
-Admitted.
+Lemma of_hexadecimal_dnorm d : of_hexadecimal (dnorm d) = of_hexadecimal d.
+Proof. now apply to_hexadecimal_inj; rewrite !to_of; [|rewrite dnorm_invol]. Qed.
 
-Lemma of_inj d d' :
-  of_hexadecimal d = of_hexadecimal d' -> hnorme d = hnorme d'.
-Admitted.
+Lemma of_inj d d' : of_hexadecimal d = of_hexadecimal d' -> dnorm d = dnorm d'.
+Proof.
+intro H.
+apply (@f_equal _ _ (fun x => match x with Some x => x | _ => d end)
+                (Some (dnorm d)) (Some (dnorm d'))).
+now rewrite <- !to_of, H.
+Qed.
 
-Lemma of_iff d d' :
-  of_hexadecimal d = of_hexadecimal d' <-> hnorme d = hnorme d'.
-Admitted.
+Lemma of_iff d d' : of_hexadecimal d = of_hexadecimal d' <-> dnorm d = dnorm d'.
+Proof.
+split. apply of_inj. intros E. rewrite <- of_hexadecimal_dnorm, E.
+apply of_hexadecimal_dnorm.
+Qed.
